examples/pseudo_bool/cp_encoding/cp_to_ilp_countingScript.sml
@@ -7,79 +7,223 @@ Libs
 Ancestors
   pbc cp ilp cp_to_ilp
 
-(* AllDifferent: All variables must take distinct values
-   For n variables, this requires O(n^2) pairwise inequality constraints *)
-Definition cencode_all_different_def:
-  cencode_all_different bnd Xs name =
+(* AllDifferentExcept, AllDifferent is just a special case *)
+
+(* Ensure that X is not in any of the iS *)
+Definition check_neqs_def:
+  check_neqs X iS =
+  MAP (λv. Neg (INL (Eq X v))) iS
+End
+
+Definition cencode_all_different_except_aux_def:
+  cencode_all_different_except_aux bnd Xs iS name =
   flat_app (MAPi (λi X.
     flat_app (MAPi (λj Y.
       if i < j
       then
+        let neqs = check_neqs X iS ++ check_neqs Y iS in
         List [
           (SOME $ mk_name name
             (toString i ^ «gt» ^ toString j),
-            bits_imply bnd [Pos (neiv name i j NONE)] (mk_gt X Y));
+            bits_imply bnd (Pos (neiv name i j NONE)::neqs) (mk_gt X Y));
           (SOME $ mk_name name
             (toString i ^ «lt» ^ toString j),
-            bits_imply bnd [Neg (neiv name i j NONE)] (mk_gt Y X))]
+            bits_imply bnd (Neg (neiv name i j NONE)::neqs) (mk_gt Y X))]
       else
         Nil) Xs)) Xs)
 End
 
-Definition encode_all_different_def:
-  encode_all_different bnd Xs name = abstr $ cencode_all_different bnd Xs name
+Definition cencode_all_different_except_def:
+  cencode_all_different_except bnd Xs iS name ec =
+  let
+    (xs,ec') = cencode_eq_grid bnd Xs iS ec
+  in
+    (Append xs
+      (cencode_all_different_except_aux bnd Xs iS name), ec')
 End
 
-Theorem encode_all_different_sem_1:
-  valid_assignment bnd wi ∧
-  ALOOKUP cs name = SOME (Counting (AllDifferent Xs)) ∧
-  all_different_sem Xs wi ⇒
-  EVERY (λx. iconstraint_sem x (wi,reify_avar cs wi))
-    (encode_all_different bnd Xs name)
+Definition encode_all_different_except_aux_def:
+  encode_all_different_except_aux bnd Xs iS name =
+  abstr (cencode_all_different_except_aux bnd Xs iS name)
+End
+
+Definition encode_all_different_except_def:
+  encode_all_different_except bnd Xs iS name =
+    encode_eq_grid bnd Xs iS ++
+    encode_all_different_except_aux bnd Xs iS name
+End
+
+Theorem EVERY_lit_check_neqs[simp]:
+  EVERY (lit wb) (check_neqs X iS) ⇔
+  ∀v. MEM v iS ⇒ ¬wb (INL (Eq X v))
 Proof
-  rw[encode_all_different_def,cencode_all_different_def,all_different_sem_def,EVERY_MEM]>>
-  gvs[MEM_FLAT,MEM_MAPi]>>
-  rename1 ‘if i < j then _ else _’>>
-  Cases_on ‘i < j’>>
-  gs[reify_avar_def,reify_flag_def]
-  >- intLib.ARITH_TAC>>
+  rw[check_neqs_def,EVERY_MAP]>>
+  rw[EVERY_MEM]
+QED
+
+Theorem EL_FILTER[local]:
+  ∀Xs n.
+  n < LENGTH Xs ∧
+  P (EL n Xs) ⇒
+  ∃m.
+    m < LENGTH (FILTER P Xs) ∧
+    EL n Xs = EL m (FILTER P Xs)
+Proof
+  Induct>>rw[]>>
+  Cases_on`n`>>gvs[]
+  >- (qexists_tac`0`>>simp[])>>
+  first_x_assum drule_all>>rw[]>>
+  qexists_tac`SUC m`>>simp[]
+QED
+
+Theorem EL_FILTER2[local]:
+  ∀Xs n n'.
+  n < n' ∧
+  n' < LENGTH Xs ∧
+  P (EL n Xs) ∧ P (EL n' Xs) ⇒
+  ∃m m'.
+    m < m' ∧
+    m' < LENGTH (FILTER P Xs) ∧
+    EL n Xs = EL m (FILTER P Xs) ∧
+    EL n' Xs = EL m' (FILTER P Xs)
+Proof
+  Induct>>rw[]>>
+  Cases_on`n`>>
+  Cases_on`n'`>>gvs[]
+  >- (
+    qexists_tac`0`>>simp[]>>
+    drule_all EL_FILTER>>rw[]>>
+    qexists_tac`SUC m`>>simp[])>>
+  first_x_assum $ drule_all>>rw[]>>
+  qexists_tac`SUC m`>>
+  qexists_tac`SUC m'`>>
+  simp[]
+QED
+
+Theorem encode_all_different_except_aux_sem_1:
+  valid_assignment bnd wi ∧
+  (ALOOKUP cs name = SOME (Counting (AllDifferentExcept Xs iS')) ∨
+  ALOOKUP cs name = SOME (Counting (SymmetricAllDifferent (Xs,start))) ∨
+  ALOOKUP cs name = SOME (Misc (Circuit Xs))) ∧
+  all_different_except_sem Xs iS wi ⇒
+  EVERY (λx. iconstraint_sem x (wi,reify_avar cs wi))
+    (encode_all_different_except_aux bnd Xs iS name)
+Proof
+  rw[encode_all_different_except_aux_def,cencode_all_different_except_aux_def,
+    all_different_except_sem_def]>>
+  simp[EVERY_MEM,MEM_MAPi,MEM_FLAT,PULL_EXISTS]>>rw[]>>
+  simp[reify_avar_def,reify_flag_def,reify_reif_def]>>
+  gvs[FILTER_MAP,o_DEF]>>
   rw[]>>
-  fs[EL_ALL_DISTINCT_EL_EQ,EL_MAP]>>
-  first_x_assum $ qspecl_then [‘i’,‘j’] assume_tac>>
+  drule_at (Pos (el 2))
+    (EL_FILTER2 |> Q.GEN `P` |> Q.ISPEC `(λx. ¬MEM (varc wi x) iS)`)>>
+  simp[]>>
+  disch_then drule_all>>
+  rw[]>>
+  gvs[EL_ALL_DISTINCT_EL_EQ,EL_MAP]>>
+  rename1`varc _ (EL xx _) + -1 * varc _ (EL yy _)`>>
+  first_x_assum(qspecl_then [`xx`,`yy`] mp_tac)>>
+  simp[]>>
   intLib.ARITH_TAC
 QED
 
-Theorem all_different_sem_aux:
+Theorem encode_all_different_except_sem_1:
+  valid_assignment bnd wi ∧
+  ALOOKUP cs name = SOME (Counting (AllDifferentExcept Xs iS')) ∧
+  all_different_except_sem Xs iS wi ⇒
+  EVERY (λx. iconstraint_sem x (wi,reify_avar cs wi))
+    (encode_all_different_except bnd Xs iS name)
+Proof
+  rw[encode_all_different_except_def,cencode_all_different_except_def]>>
+  simp[reify_avar_def,reify_flag_def,reify_reif_def]>>
+  simp[encode_all_different_except_aux_sem_1]
+QED
+
+Theorem FILTER_EL[local]:
+  ∀Xs n.
+  n < LENGTH (FILTER P Xs) ⇒
+  ∃m.
+    m < LENGTH Xs ∧
+    EL m Xs = EL n (FILTER P Xs) ∧
+    P (EL m Xs)
+Proof
+  Induct>>rw[]>>
+  Cases_on`n`>>gvs[]
+  >- (qexists_tac`0`>>simp[])>>
+  first_x_assum drule_all>>rw[]>>
+  qexists_tac`SUC m`>>gvs[]
+QED
+
+Theorem FILTER_EL2[local]:
+  ∀Xs n n'.
+  n < n' ∧
+  n' < LENGTH (FILTER P Xs) ⇒
+  ∃m m'.
+    m < m' ∧
+    m' < LENGTH Xs ∧
+    EL m Xs = EL n (FILTER P Xs) ∧
+    EL m' Xs = EL n' (FILTER P Xs) ∧
+    P (EL m Xs) ∧ P (EL m' Xs)
+Proof
+  Induct>>rw[]
+  >- (
+    Cases_on`n`>>
+    Cases_on`n'`>>gvs[]
+    >- (
+      qexists_tac`0`>>simp[]>>
+      drule_all FILTER_EL>>rw[]>>
+      qexists_tac`SUC m`>>gvs[])
+    >- (
+      first_x_assum $ drule_all>>rw[]>>
+      qexists_tac`SUC m`>>
+      qexists_tac`SUC m'`>>
+      gvs[]))>>
+  first_x_assum drule_all>>rw[]>>
+  qexists_tac`SUC m`>>
+  qexists_tac`SUC m'`>>
+  gvs[]
+QED
+
+Theorem all_different_except_sem_imp:
   (∀i j. i < j ∧ j < LENGTH Xs ⇒
     let X = EL i Xs in
     let Y = EL j Xs in
-    if wb (neiv (name:mlstring) i j NONE)
-    then varc wi X > varc wi Y
-    else varc wi Y > varc wi X) ⇒
-  all_different_sem Xs wi
+    if (wb:'a avar -> bool) (neiv (name:mlstring) i j NONE)
+    then ¬ MEM (varc wi X) iS ∧  ¬ MEM (varc wi Y) iS ⇒ varc wi X > varc wi Y
+    else ¬ MEM (varc wi X) iS ∧  ¬ MEM (varc wi Y) iS ⇒ varc wi Y > varc wi X) ⇒
+  all_different_except_sem Xs iS wi
 Proof
-  rw[all_different_sem_def,EL_ALL_DISTINCT_EL_EQ]>>
+  rw[all_different_except_sem_def,EL_ALL_DISTINCT_EL_EQ]>>
   Cases_on`n1 = n2`>>simp[]>>
   wlog_tac `n1 < n2` [`n1`,`n2`]
   >- (
     `n2 < n1` by fs[]>>
-    first_x_assum drule_all>>
-    simp[])>>
-  first_x_assum drule>>
-  rw[EL_MAP]>>
+    first_x_assum drule>>simp[])>>
+  drule_all FILTER_EL2>>
+  rw[]>>
+  first_x_assum drule_all>>gvs[EL_MAP]>>rw[]>>
   intLib.ARITH_TAC
 QED
 
-Theorem encode_all_different_sem_2:
+Theorem encode_all_different_except_aux_sem_2:
   valid_assignment bnd wi ∧
+  (∀X i.
+    MEM X Xs ∧ MEM i iS ⇒
+    (wb (INL (Ge X i)) ⇔ varc wi X ≥ i) ∧
+    (wb (INL (Ge X (i + 1))) ⇔ varc wi X ≥ i + 1) ∧
+    (wb (INL (Eq X i)) ⇔ varc wi X = i)) ∧
   EVERY (λx. iconstraint_sem x (wi,wb))
-    (encode_all_different bnd Xs name) ⇒
-  all_different_sem Xs wi
+    (encode_all_different_except_aux bnd Xs iS name) ⇒
+  all_different_except_sem Xs iS wi
 Proof
   strip_tac>>
-  irule all_different_sem_aux>>
-  gs[EVERY_MEM,encode_all_different_def,cencode_all_different_def,
-    MEM_FLAT,MEM_MAPi,PULL_EXISTS]>>
+  irule all_different_except_sem_imp>>
+  gs[encode_all_different_except_def]>>
+  pop_assum mp_tac>>
+  simp[EVERY_MEM,cencode_all_different_except_aux_def,
+    encode_all_different_except_aux_def,
+    MEM_FLAT,MEM_MAPi,PULL_EXISTS,SF DNF_ss]>>
+  rw[]>>
   qexistsl [‘name’,‘wb’]>>
   rpt strip_tac>>
   rename1 ‘[i;j]’>>
@@ -87,12 +231,264 @@ Proof
   first_x_assum $ drule_then rev_drule>>
   simp[SF DNF_ss]>>
   rw[]>>
-  intLib.ARITH_TAC
+  qpat_x_assum`_ ⇒ _` mp_tac>>
+  (* two subgoals*)
+  (reverse impl_tac >- intLib.ARITH_TAC)>>
+  rw[]>>
+  gvs[MEM_EL,PULL_EXISTS]>>
+  first_x_assum (drule_at (Pos last))>>rw[]>>
+  first_assum (qspec_then`i` mp_tac)>>
+  first_x_assum (qspec_then`j` mp_tac)>>
+  simp[]>>
+  CCONTR_TAC>>gvs[]
 QED
 
-(* TODO: AllDifferentExcept *)
+Theorem encode_all_different_except_sem_2:
+  valid_assignment bnd wi ∧
+  EVERY (λx. iconstraint_sem x (wi,wb))
+    (encode_all_different_except bnd Xs iS name) ⇒
+  all_different_except_sem Xs iS wi
+Proof
+  strip_tac>>
+  irule encode_all_different_except_aux_sem_2>>
+  gs[encode_all_different_except_def]>>
+  metis_tac[]
+QED
 
-(* TODO: SymmetricAllDifferent *)
+Theorem cencode_all_different_except_sem:
+  valid_assignment bnd wi ∧
+  cencode_all_different_except bnd Xs iS name ec = (es, ec') ⇒
+  enc_rel wi es (encode_all_different_except bnd Xs iS name) ec ec'
+Proof
+  rw[cencode_all_different_except_def,encode_all_different_except_def]>>
+  gvs[AllCaseEqs(),UNCURRY_EQ]>>
+  irule enc_rel_Append>>
+  irule_at Any enc_rel_encode_eq_grid>>simp[]>>
+  simp[encode_all_different_except_aux_def]
+QED
+
+(* These are convenient because they are reused *)
+Definition cencode_all_different_def:
+  cencode_all_different bnd Xs name =
+  cencode_all_different_except_aux bnd Xs [] name
+End
+
+Definition encode_all_different_def:
+  encode_all_different bnd Xs name =
+  encode_all_different_except_aux bnd Xs [] name
+End
+
+Theorem encode_all_different_sem_1:
+  valid_assignment bnd wi ∧
+  (ALOOKUP cs name = SOME (Counting (AllDifferentExcept Xs iS)) ∨
+  ALOOKUP cs name = SOME (Counting (SymmetricAllDifferent (Xs,start))) ∨
+  ALOOKUP cs name = SOME (Misc (Circuit Xs))) ∧
+  all_different_except_sem Xs [] wi ⇒
+  EVERY (λx. iconstraint_sem x (wi,reify_avar cs wi))
+    (encode_all_different bnd Xs name)
+Proof
+  rw[encode_all_different_def]>>
+  irule encode_all_different_except_aux_sem_1>>
+  simp[]
+QED
+
+Theorem encode_all_different_sem_2:
+  valid_assignment bnd wi ∧
+  EVERY (λx. iconstraint_sem x (wi,wb))
+    (encode_all_different bnd Xs name) ⇒
+  all_different_except_sem Xs [] wi
+Proof
+  rw[encode_all_different_def]>>
+  irule encode_all_different_except_aux_sem_2>>
+  simp[]>>
+  metis_tac[]
+QED
+
+Theorem encode_all_different_alt:
+  encode_all_different bnd Xs name =
+  abstr (cencode_all_different bnd Xs name)
+Proof
+  rw[cencode_all_different_def,encode_all_different_def,
+    encode_all_different_except_aux_def]
+QED
+
+(* TODO: move, perhaps generalize? *)
+Definition cmk_bounds_def:
+  cmk_bounds name tag X a b =
+  List
+  (mk_annotate
+    [mk_name name (tag ^ «_lb»);mk_name name (tag ^ «_ub»)]
+    (mk_bounds X a b))
+End
+
+(* Give uniform bound lb ≤ Xs ≤ ub *)
+Definition cmk_bounds_all_def:
+  cmk_bounds_all name Xs lb ub =
+  flat_app
+    (MAPi
+      (λi X.
+        cmk_bounds name («X_» ^ toString (i+1)) X lb ub) Xs)
+End
+
+Theorem cmk_bounds_all_sem:
+  EVERY (λx. iconstraint_sem x (wi,wb))
+    (abstr (cmk_bounds_all name Xs lb ub)) ⇔
+  (∀X. MEM X Xs ⇒
+    varc wi X ≥ lb ∧ varc wi X ≤ ub)
+Proof
+  rw[cmk_bounds_all_def,EVERY_FLAT]>>
+  simp[Once EVERY_MEM,MEM_MAPi]>>
+  simp[PULL_EXISTS,cmk_bounds_def,MEM_EL]
+QED
+
+Definition cencode_symmetric_all_different_aux_def:
+  cencode_symmetric_all_different_aux bnd Xs start name =
+  let n = LENGTH Xs in
+  Append
+  (* All different *)
+  (cencode_all_different bnd Xs name)
+  (* Range *)
+  (Append (cmk_bounds_all name Xs start (start + &n -1))
+  (* Involution *)
+  (flat_app (MAPi (λi X.
+    flat_app (MAPi (λj Y.
+      if i < j
+      then
+        (* Xs[i]={j+start} ⇒ Xs[j]={i+start} *)
+        cbimply_var bnd (INL (Eq X (&j + start)))
+          ([],[(1, Pos (INL (Eq Y (&i + start))))],1)
+      else
+        Nil) Xs)) Xs)))
+End
+
+Definition cencode_symmetric_all_different_def:
+  cencode_symmetric_all_different bnd Xs start name ec =
+  let
+    n = LENGTH Xs;
+    (xs,ec') = cencode_eq_grid bnd Xs (GENLIST (λi. start + &i) n) ec
+  in
+    (Append xs
+      (cencode_symmetric_all_different_aux bnd Xs start name), ec')
+End
+
+Definition encode_symmetric_all_different_def:
+  encode_symmetric_all_different bnd Xs start name =
+  let
+    n = LENGTH Xs;
+  in
+    encode_eq_grid bnd Xs (GENLIST (λi. start + &i) n) ++
+      (abstr (cencode_symmetric_all_different_aux bnd Xs start name))
+End
+
+Theorem symmetric_all_different_sem_alt:
+  symmetric_all_different_sem (Xs,start) w ⇔
+  let n = LENGTH Xs in
+    ALL_DISTINCT (MAP (varc w) Xs) ∧
+    EVERY (λX. start ≤ varc w X ∧ varc w X < start + &n) Xs ∧
+    (∀i j. i < n ∧ j < n ⇒
+      (varc w (EL i Xs) = &j + start
+      ⇔
+      varc w (EL j Xs) = &i + start))
+Proof
+  rw[symmetric_all_different_sem_def]>>eq_tac>>
+  rw[]
+  >- (
+    rw[EL_ALL_DISTINCT_EL_EQ]>>
+    eq_tac>>rw[]>>
+    gvs[EL_MAP]>>
+    first_assum(qspec_then `n1` mp_tac)>>
+    first_x_assum(qspec_then `n2` mp_tac)>>
+    simp[])
+  >- (
+    first_assum(qspec_then `i` mp_tac)>>
+    first_x_assum(qspec_then `j` mp_tac)>>
+    rw[]>>eq_tac>>rw[]>>gvs[]>>
+    `∀n.Num (&n + start − start) = n` by intLib.ARITH_TAC>>
+    gvs[])
+  >- (
+    gvs[EVERY_EL]>>last_x_assum drule>>rw[]>>
+    first_x_assum(qspecl_then[`i`,`Num (varc w Xs❲i❳ − start)`] mp_tac)>>
+    simp[]>>
+    intLib.ARITH_TAC)
+QED
+
+Theorem encode_symmetric_all_different_sem_1:
+  valid_assignment bnd wi ∧
+  ALOOKUP cs name = SOME (Counting (SymmetricAllDifferent (Xs,start))) ∧
+  symmetric_all_different_sem (Xs,start) wi ⇒
+  EVERY (λx. iconstraint_sem x (wi,reify_avar cs wi))
+    (encode_symmetric_all_different bnd Xs start name)
+Proof
+  rw[encode_symmetric_all_different_def,cencode_symmetric_all_different_def,
+    symmetric_all_different_sem_alt]>>
+  simp[reify_avar_def,reify_flag_def,reify_reif_def]>>
+  simp[cencode_symmetric_all_different_aux_def]>>rw[]
+  >- (
+    (* all different *)
+    simp[GSYM encode_all_different_alt]>>
+    irule encode_all_different_sem_1>>
+    simp[all_different_except_sem_def])
+  >- (
+    (* range *)
+    fs[cmk_bounds_all_sem,EVERY_MEM]>>
+    rw[]>>first_x_assum drule>>
+    rpt (pop_assum kall_tac)>>
+    intLib.ARITH_TAC)>>
+  (* involution *)
+  simp[EVERY_FLAT,Once EVERY_MEM]>>
+  simp[MEM_FLAT,MEM_MAPi,PULL_EXISTS,EVERY_FLAT]>>
+  simp[Once EVERY_MEM,MEM_MAPi]>>rw[]>>rw[]>>
+  simp[iconstraint_sem_def,reify_avar_def,reify_reif_def,oneline b2i_def]>>
+  rw[]
+QED
+
+Theorem encode_symmetric_all_different_sem_2:
+  valid_assignment bnd wi ∧
+  EVERY (λx. iconstraint_sem x (wi,wb))
+    (encode_symmetric_all_different bnd Xs start name) ⇒
+  symmetric_all_different_sem (Xs,start) wi
+Proof
+  rw[symmetric_all_different_sem_alt,encode_symmetric_all_different_def,
+    cencode_symmetric_all_different_aux_def]
+  >- (
+    gvs[GSYM (encode_all_different_alt)]>>
+    drule_all encode_all_different_sem_2>>
+    simp[all_different_except_sem_def])
+  >- (
+    (* range *)
+    fs[cmk_bounds_all_sem,EVERY_MEM]>>
+    rw[]>>first_x_assum drule>>
+    rpt (pop_assum kall_tac)>>
+    intLib.ARITH_TAC)>>
+  (* involution *)
+  qpat_x_assum`EVERY _ (FLAT _)` mp_tac>>
+  simp[EVERY_FLAT,Once EVERY_MEM]>>
+  simp[MEM_FLAT,MEM_MAPi,PULL_EXISTS,EVERY_FLAT]>>
+  simp[Once EVERY_MEM,MEM_MAPi,PULL_EXISTS,PULL_FORALL]>>
+  Cases_on`i=j`>>simp[]>>
+  wlog_tac `i < j` [`i`,`j`]
+  >- (
+    `j < i` by fs[]>>
+    first_x_assum drule>>simp[])>>
+  disch_then (qspecl_then[`i`,`j`] mp_tac)>>
+  simp[iconstraint_sem_def,reify_avar_def,reify_reif_def,oneline b2i_def]>>
+  gvs[MEM_GENLIST,PULL_EXISTS,MEM_EL]>>
+  first_assum (qspecl_then [`i`,`j`] mp_tac)>>
+  first_x_assum (qspecl_then [`j`,`i`] mp_tac)>>
+  rw[]>>
+  metis_tac[integerTheory.INT_ADD_COMM]
+QED
+
+Theorem cencode_symmetric_all_different_sem:
+  valid_assignment bnd wi ∧
+  cencode_symmetric_all_different bnd Xs iS name ec = (es, ec') ⇒
+  enc_rel wi es (encode_symmetric_all_different bnd Xs iS name) ec ec'
+Proof
+  rw[cencode_symmetric_all_different_def,encode_symmetric_all_different_def]>>
+  gvs[AllCaseEqs(),UNCURRY_EQ]>>
+  irule enc_rel_Append>>
+  irule_at Any enc_rel_encode_eq_grid>>simp[]
+QED
 
 Definition elm_def[simp]:
   elm name (v:int) =
@@ -159,7 +555,7 @@ Definition encode_n_value_def:
   let
     vals = union_dom bnd Xs
   in
-    FLAT (MAP (λv. FLAT (MAP (λX. encode_full_eq bnd X v) Xs)) vals) ++
+    encode_eq_grid bnd Xs vals ++
     FLAT (MAP (λv. encode_some_eq bnd Xs v name) vals) ++
     encode_bitsum (MAP (elm name) vals) Y
 End
@@ -177,14 +573,21 @@ Theorem encode_n_value_aux:
 Proof
   strip_tac>>
   simp[encode_n_value_def]>>
-  ntac 2 (simp[EVERY_FLAT,EVERY_MAP])>>
-  simp[GSYM EVERY_CONJ,Once EVERY_MEM]>>
-  simp[EVERY_CONJ, Once $ METIS_PROVE[]
-    “(P1 ∧ P2 ∧ P3) ∧ P4 ⇔ (P1 ∧ P2 ∧ P3) ∧ (P3 ⇒ P4)”]>>
-  drule_then (fn thm => simp[thm]) encode_bitsum_sem>>
-  simp[MAP_MAP_o]>>
-  simp[iSUM_FILTER,o_DEF,encode_some_eq_sem,MEM_MAP,EVERY_MEM]>>
-  metis_tac[]
+  irule LEFT_AND_CONG>>rw[]
+  >- (
+    simp[IMP_CONJ_THM, SF DNF_ss]>>
+    simp[CONJ_ASSOC]>>
+    irule LEFT_AND_CONG>>rw[]
+    >- (
+      simp[EVERY_MEM]>>metis_tac[])>>
+    simp[EVERY_FLAT,Once EVERY_MEM,MEM_MAP,PULL_EXISTS]>>
+    drule encode_some_eq_sem>>
+    fs[EVERY_MEM]>>
+    metis_tac[])
+  >- (
+    drule_then (fn thm => simp[thm]) encode_bitsum_sem>>
+    simp[MAP_MAP_o]>>
+    simp[iSUM_FILTER,o_DEF,encode_some_eq_sem,MEM_MAP,EVERY_MEM])
 QED
 
 Theorem encode_n_value_sem_1:
@@ -248,9 +651,7 @@ Definition cencode_n_value_def:
   cencode_n_value bnd Xs Y name ec =
   let
     vals = union_dom bnd Xs;
-    (xs,ec') =
-      fold_cenc (λv ec.
-        fold_cenc (λX ec. cencode_full_eq bnd X v ec) Xs ec) vals ec
+    (xs,ec') = cencode_eq_grid bnd Xs vals ec
   in
     (Append
       (Append xs
@@ -273,25 +674,7 @@ Proof
   >-(
     irule enc_rel_Append>>
     qexists ‘ec'’>>
-    CONJ_TAC
-    >-(
-      pop_assum mp_tac>>
-      qmatch_goalsub_abbrev_tac
-        ‘fold_cenc cf _ _ = _ ⇒ enc_rel _ _ (FLAT (MAP f _)) _ _’>>
-      rename1 ‘fold_cenc _ ls _’>>
-      qid_spec_tac ‘ec'’>>
-      qid_spec_tac ‘xs’>>
-      qid_spec_tac ‘ec’>>
-      qid_spec_tac ‘ls’>>
-      ho_match_mp_tac enc_rel_fold_cenc>>
-      simp[Abbr‘cf’,Abbr‘f’]>>
-      strip_tac>>
-      qmatch_goalsub_abbrev_tac
-        ‘fold_cenc cf _ _ = _ ⇒ enc_rel _ _ (FLAT (MAP f _)) _ _’>>
-      qid_spec_tac ‘Xs’>>
-      ho_match_mp_tac enc_rel_fold_cenc>>
-      simp[Abbr‘cf’,Abbr‘f’]>>
-      metis_tac[enc_rel_encode_full_eq])>>
+    simp[enc_rel_encode_eq_grid]>>
     irule enc_rel_abstr_cong>>
     simp[abstr_flat_app,encode_some_eq_def,MAP_MAP_o,o_DEF])>>
   simp[cencode_bitsum_def]
@@ -330,10 +713,7 @@ End
 Definition cencode_in_def:
   cencode_in bnd (Xs:mlstring varc list) Y name ec =
   let (Xsv,Xsc) = split_varc_in_list Xs in
-  let (cs_enc,ec') =
-    fold_cenc
-      (λc ec. cencode_full_eq bnd Y c ec)
-      Xsc ec in
+  let (cs_enc,ec') = cencode_eq_grid bnd [Y] Xsc ec in
   let var_lits =
     GENLIST (λi. Pos $ eqi name i («eq»)) (LENGTH Xsv) in
   let con_lits =
@@ -346,7 +726,7 @@ End
 Definition encode_in_def:
   encode_in bnd (Xs:mlstring varc list) Y name =
   let (Xsv,Xsc) = split_varc_in_list Xs in
-  FLAT (MAP (λc. encode_full_eq bnd Y c) Xsc) ++
+  encode_eq_grid bnd [Y] Xsc ++
   abstr (cencode_count_aux bnd Xsv Y name) ++
   [at_least_one
     (GENLIST (λi. Pos $ eqi name i («eq»)) (LENGTH Xsv) ++
@@ -429,10 +809,8 @@ Theorem encode_in_sem_1:
     (encode_in bnd Xs Y name)
 Proof
   rw[encode_in_def,in_sem_def]>>
-  pairarg_tac>>rw[]
-  >- (
-    simp[EVERY_FLAT,EVERY_MAP,Once EVERY_MEM]>>
-    Cases>>rw[reify_avar_def,reify_reif_def])
+  pairarg_tac>>rw[]>>
+  simp[reify_avar_def,reify_reif_def]
   >- (
     irule encode_count_aux_sem_1>>
     gvs[]>>
@@ -561,21 +939,7 @@ Proof
   gvs[AllCaseEqs(),UNCURRY_EQ]>>
   PURE_ONCE_REWRITE_TAC[GSYM APPEND_ASSOC]>>
   irule enc_rel_Append>>
-  rename1 ‘_ = (xs,_)’>>
-  qexists ‘ec'’>>
-  CONJ_TAC
-  >-(
-    pop_assum mp_tac>>
-    qmatch_goalsub_abbrev_tac
-      ‘fold_cenc cf _ _ = _ ⇒ enc_rel _ _ (FLAT (MAP f _)) _ _’>>
-    rename1 ‘fold_cenc _ ls _’>>
-    qid_spec_tac ‘ec'’>>
-    qid_spec_tac ‘xs’>>
-    qid_spec_tac ‘ec’>>
-    qid_spec_tac ‘ls’>>
-    ho_match_mp_tac enc_rel_fold_cenc>>
-    simp[Abbr‘cf’,Abbr‘f’]>>
-    metis_tac[enc_rel_encode_full_eq])>>
+  irule_at Any enc_rel_encode_eq_grid>>simp[]>>
   irule enc_rel_abstr_cong>>
   simp[]
 QED
@@ -591,8 +955,7 @@ End
 
 Definition encode_among_def:
   encode_among bnd Xs iS Y name =
-  FLAT (MAP (λX.
-    FLAT (MAP (λv. encode_full_eq bnd X v) iS)) Xs) ++
+  encode_eq_grid bnd Xs iS ++
   abstr (cencode_among_aux bnd Xs iS Y name)
 End
 
@@ -614,11 +977,8 @@ Theorem encode_among_sem_1:
   EVERY (λx. iconstraint_sem x (wi,reify_avar cs wi))
     (encode_among bnd Xs iS Y name)
 Proof
-  rw[cencode_among_aux_def,encode_among_def,among_sem_def]
-  >-(
-    simp[EVERY_FLAT,Once EVERY_MEM,MEM_MAP,PULL_EXISTS]>>
-    rw[Once EVERY_MEM,MEM_MAP]>>
-    simp[reify_avar_def,reify_reif_def])>>
+  rw[cencode_among_aux_def,encode_among_def,among_sem_def]>>
+  simp[reify_avar_def,reify_reif_def]>>
   drule_then (fn thm => simp[thm]) encode_bitsum_sem>>
   simp[MAP_FLAT,pbc_encodeTheory.iSUM_FLAT,MAP_MAP_o,o_DEF]>>
   rw[reify_avar_def,reify_reif_def]>>
@@ -637,62 +997,16 @@ Proof
   rw[cencode_among_aux_def,encode_among_def,EVERY_FLAT,among_sem_def]>>
   drule_then (fn thm => gs[thm]) encode_bitsum_sem>>
   pop_assum (SUBST_ALL_TAC o SYM)>>
-  qpat_x_assum`EVERY _ _` mp_tac>>
-  simp[Once EVERY_MEM,MEM_MAPi,SF DNF_ss,iconstraint_sem_def,EVERY_FLAT,EVERY_MAP,MEM_MAP]>>
-  rw[]>>
   simp[MAP_FLAT,pbc_encodeTheory.iSUM_FLAT,MAP_MAP_o,o_DEF]>>
   cong_tac NONE>>
   PURE_REWRITE_TAC[Once (GSYM MEM_nub)]>>
   ho_match_mp_tac iSUM_ALL_DISTINCT_MEM>>
-  rw[]>>
-  first_x_assum drule_all>>rw[EVERY_MEM]
-QED
-
-(* (encode_full_eq_ilist bnd X iS) extends (encode_full_eq bnd X v)
-   from a single int ‘v’ to an int list ‘iS’ *)
-Definition encode_full_eq_ilist_def:
-  encode_full_eq_ilist bnd _ [] = [] ∧
-  encode_full_eq_ilist bnd X (i::iS) =
-    encode_full_eq bnd X i ++ encode_full_eq_ilist bnd X iS
-End
-
-Definition cencode_full_eq_ilist_def:
-  cencode_full_eq_ilist bnd X [] ec = (Nil,ec) ∧
-  cencode_full_eq_ilist bnd X (i::iS) ec =
-  let
-    (x1,ec') = cencode_full_eq bnd X i ec;
-    (x2,ec'') = cencode_full_eq_ilist bnd X iS ec'
-  in
-    (Append x1 x2,ec'')
-End
-
-Theorem cencode_full_eq_ilist_sem:
-  ∀es ec. valid_assignment bnd wi ∧
-  cencode_full_eq_ilist bnd X iS ec = (es, ec') ⇒
-    enc_rel wi es (encode_full_eq_ilist bnd X iS) ec ec'
-Proof
-  Induct_on ‘iS’>>
-  rw[cencode_full_eq_ilist_def,encode_full_eq_ilist_def]>>
-  rpt (pairarg_tac>>fs[])>>
-  ntac 2 (last_x_assum mp_tac)>>
-  last_x_assum (SUBST_ALL_TAC o SYM)>>
-  last_x_assum SUBST_ALL_TAC>>
-  rpt strip_tac>>
-  irule enc_rel_Append>>
-  rename1 ‘cencode_full_eq _ _ _ _ = (_,ec0)’>>
-  qexists ‘ec0’>>
-  CONJ_TAC
-  >-(
-    irule enc_rel_encode_full_eq>>
-    simp[])>>
-  metis_tac[]
+  rw[]
 QED
 
 Definition cencode_among_def:
   cencode_among bnd Xs iS Y name ec =
-  let (xs,ec') =
-    fold_cenc (λX ec.
-      fold_cenc (λv ec. cencode_full_eq bnd X v ec) iS ec) Xs ec in
+  let (xs,ec') = cencode_eq_grid bnd Xs iS ec in
   (Append xs (cencode_among_aux bnd Xs iS Y name), ec')
 End
 
@@ -705,14 +1019,7 @@ Proof
   gvs[AllCaseEqs(),UNCURRY_EQ]>>
   irule enc_rel_Append>>
   irule_at Any enc_rel_abstr>>
-  irule enc_rel_fold_cenc>>
-  first_x_assum $ irule_at Any>>
-  rw[]>>
-  irule enc_rel_fold_cenc>>
-  first_x_assum $ irule_at Any>>
-  rw[]>>
-  irule enc_rel_encode_full_eq>>
-  fs[]
+  simp[enc_rel_encode_eq_grid]
 QED
 
 (* AllEqual: linear chain x1=x2, x2=x3, ... *)
@@ -771,33 +1078,10 @@ Proof
   simp[Once EQ_SYM_EQ]
 QED
 
-(* TODO: AllDifferentExcept *)
-Definition cencode_all_different_except_def:
-  cencode_all_different_except bnd Xs (iS:int list) name =
-  Nil
-End
-
-Definition encode_all_different_except_def:
-  encode_all_different_except bnd Xs iS name =
-  []
-End
-
-(* TODO: SymmetricAllDifferent *)
-Definition cencode_symmetric_all_different_def:
-  cencode_symmetric_all_different bnd Xs start name ec =
-  (Nil,ec)
-End
-
-Definition encode_symmetric_all_different_def:
-  encode_symmetric_all_different bnd Xs start name =
-  []
-End
-
 Definition encode_counting_constr_def:
   encode_counting_constr bnd c name =
   case c of
     AllEqual Xs => encode_all_equal Xs name
-  | AllDifferent Xs => encode_all_different bnd Xs name
   | AllDifferentExcept Xs iS => encode_all_different_except bnd Xs iS name
   | SymmetricAllDifferent (Xs,start) => encode_symmetric_all_different bnd Xs start name
   | NValue Xs Y => encode_n_value bnd Xs Y name
@@ -817,9 +1101,8 @@ Proof
   Cases_on`c`>>
   rw[encode_counting_constr_def,counting_constr_sem_def]
   >- metis_tac[encode_all_equal_sem_1]
-  >- metis_tac[encode_all_different_sem_1]
-  >- cheat (* AllDifferentExcept *)
-  >- cheat (* SymmetricAllDifferent *)
+  >- metis_tac[encode_all_different_except_sem_1]
+  >- (Cases_on`p`>>fs[]>>metis_tac[encode_symmetric_all_different_sem_1])
   >- metis_tac[encode_n_value_sem_1]
   >- metis_tac[encode_count_sem_1]
   >- metis_tac[encode_among_sem_1]
@@ -836,9 +1119,8 @@ Proof
   Cases_on`c`>>
   rw[encode_counting_constr_def,counting_constr_sem_def]
   >- metis_tac[encode_all_equal_sem_2]
-  >- metis_tac[encode_all_different_sem_2]
-  >- cheat (* AllDifferentExcept *)
-  >- cheat (* SymmetricAllDifferent *)
+  >- metis_tac[encode_all_different_except_sem_2]
+  >- (Cases_on`p`>>fs[]>>metis_tac[encode_symmetric_all_different_sem_2])
   >- metis_tac[encode_n_value_sem_2]
   >- metis_tac[encode_count_sem_2]
   >- metis_tac[encode_among_sem_2]
@@ -850,8 +1132,7 @@ Definition cencode_counting_constr_def:
   cencode_counting_constr bnd c name ec =
   case c of
     AllEqual Xs => (cencode_all_equal Xs name, ec)
-  | AllDifferent Xs => (cencode_all_different bnd Xs name, ec)
-  | AllDifferentExcept Xs iS => (cencode_all_different_except bnd Xs iS name, ec)
+  | AllDifferentExcept Xs iS => cencode_all_different_except bnd Xs iS name ec
   | SymmetricAllDifferent (Xs,start) => cencode_symmetric_all_different bnd Xs start name ec
   | NValue Xs Y => cencode_n_value bnd Xs Y name ec
   | Count Xs Y Z => (cencode_count bnd Xs Y Z name, ec)
@@ -868,9 +1149,8 @@ Proof
   Cases_on ‘c’>>
   simp[cencode_counting_constr_def,encode_counting_constr_def]
   >- simp[cencode_all_equal_def,encode_all_equal_def]
-  >- simp[cencode_all_different_def,encode_all_different_def]
-  >- cheat (* AllDifferentExcept *)
-  >- cheat (* SymmetricAllDifferent *)
+  >- simp[cencode_all_different_except_sem]
+  >- (Cases_on`p`>>simp[cencode_symmetric_all_different_sem])
   >- simp[cencode_n_value_sem]
   >- simp[cencode_count_def,encode_count_def]
   >- simp[cencode_among_sem]
